another transition

concurrency/scache/RWLock.i.dfy
@@ -573,30 +573,46 @@ module RWLockExt refines SimpleExt {
     assert dot(m', p).sharedState == dot(m, p).sharedState;
   }
 
+  predicate ReadingIncCount(m: M, m': M, t: int)
+  {
+    && t in m.refCounts
+    && 0 <= t < NUM_THREADS
+    && m == dot(
+      ReadHandle(ReadPending),
+      RefCount(t, m.refCounts[t])
+    )
+    && m' == dot(
+      ReadHandle(ReadPendingCounted(t)),
+      RefCount(t, m.refCounts[t] + 1)
+    )
+  }
+
+  lemma ReadingIncCount_Preserves(p: M, m: M, m': M, t: int)
+  requires dot_defined(m, p)
+  requires Inv(dot(m, p))
+  requires ReadingIncCount(m, m', t)
+  ensures dot_defined(m', p)
+  ensures Inv(dot(m', p))
+  ensures Interp(dot(m, p)) == Interp(dot(m', p))
+  {
+    SumFilterSimp<SharedState>();
+    assert dot(m', p).sharedState == dot(m, p).sharedState;
+    var state := dot(m, p);
+    var state' := dot(m', p);
+    forall t0 | 0 <= t0 < NUM_THREADS
+    ensures t0 in state'.refCounts && state'.refCounts[t0] == CountAllRefs(state', t0)
+    {
+      if t == t0 {
+        assert CountAllRefs(state', t0) == CountAllRefs(state, t0) + 1;
+        assert t0 in state'.refCounts && state'.refCounts[t0] == CountAllRefs(state', t0);
+      } else{
+        assert CountAllRefs(state', t0) == CountAllRefs(state, t0);
+        assert t0 in state'.refCounts && state'.refCounts[t0] == CountAllRefs(state', t0);
+      }
+    }
+  }
 
   /*
-
-  predicate ReadingIncCount(
-    key: Key, state: RWLockState, state': RWLockState,
-    a: multiset<R>, a': multiset<R>,
-    client: R, rc: R, r: R, rc': R, r': R, t: int, refcount: uint8)
-  {
-    && a == multiset{rc, r, client}
-    && a' == multiset{rc', r'}
-    && (0 <= t < |state.readCounts| ==>
-        state' == state
-          .(readCounts := state.readCounts[t := state.readCounts[t] + 1])
-          .(readState := RSPendingCounted(t))
-    )
-    && rc == Internal(SharedLockRefCount(key, t, refcount))
-    && r == Internal(ReadingPending(key))
-    && client == Internal(Client(t))
-    && rc' == Internal(SharedLockRefCount(key, t,
-        // uint8 addition
-        // (we'll need to prove invariant that this doesn't overflow)
-        if refcount == 255 then 0 else refcount + 1))
-    && r' == Internal(ReadingPendingCounted(key, t))
-  }
 
   predicate ObtainReading(
     key: Key, state: RWLockState, state': RWLockState,
